wip

code/rocq/check.v
@@ -129,17 +129,40 @@ Module check (U:Unif).
   Fixpoint has_cut_and A :=
     match A with
     | Goal _ Cut => true
+    | KO => true
     | And A _ B => has_cut_and A || has_cut_and B
     | _ => false
     end.
 
+  Lemma has_cut_and_has_cut_and_cut {B}: has_cut_and B -> has_cut_and (cut B).
+  Proof.
+    elim:B => // A HA B HB C HC /=/orP[].
+    (* + by move=> /HA ->.
+    + by move=> /HC ->; rewrite orbT. *)
+  Qed.
+
   Fixpoint has_cut_or A :=
     match A with
     | Or A _ B => has_cut_and A && has_cut_or B
-    | _ => false
+    | _ => has_cut_and A
     end.
 
-  Definition has_cut A := match A with KO => true | Or KO _ A => has_cut_or A | _ => false end.
+  Definition has_cut A := match A with KO | Goal _ Cut => true| And _ _ _ => has_cut_and A | Or _ _ _ => has_cut_or A | _ => false end.
+
+  Lemma has_cut_or_has_cut {A}: has_cut_or A -> has_cut A.
+  Proof. elim: A => - // [] //. Qed.
+
+  Lemma has_cut_and_has_cut {A}: has_cut_and A -> has_cut A.
+  Proof. elim: A => //. Qed.
+
+  Lemma has_cut_or_has_cut_or_cut {B}: has_cut_or B -> has_cut_or (cut B).
+  Proof.
+    elim:B => //= [] // [] //.
+    (* + by move=> ? [] //.
+    + by move=> A B C H _ D H1 /andP[] /= /orP [] /has_cut_and_has_cut_and_cut -> /H1 -> //; rewrite orbT//.
+    + by move=> A s B HB C HC D HD /orP [] /has_cut_and_has_cut_and_cut -> //; rewrite orbT//. *)
+    (* + move=> A B C HA D HD E HE /orP [] /has_cut_and_has_cut_and_cut -> //; rewrite orbT//. *)
+  Qed.
 
   Fixpoint no_new_alt_aux A :=
     match A with
@@ -149,12 +172,22 @@ Module check (U:Unif).
     | Top | Bot | Goal _ _ | KO => true
     end.
 
+    Definition det_rule_cut (r : R) :=
+    match r.(premises) with [::] => false | x :: xs => last x xs == Cut end.
+
   Fixpoint no_new_alt sold snew :=   
     match sold, snew with
     | OK, OK | KO, KO | Top, Top | Top, OK | Bot, Bot | Bot, KO => true
-    | Or A _ B, Or A' _ B' => (no_new_alt A A') && ((B == B') || (cut B == B'))
-    | And A _ B, And A' _ B' => no_new_alt A A' && no_new_alt B B'
-    | Goal _ _, snew => (*has_cut snew || *) no_new_alt_aux snew
+    | _, KO => true
+    | Or A _ B, Or A' _ B' =>
+    (* To be checked, because, when we backtrack, we remove A from the new state, and therefore,
+      sold could be A \/ B and snew could be B' *)
+      (* if success A then (no_new_alt A A') && ((B == B') || (cut B == B'))
+      else failed A && no_new_alt B B' *)
+      no_new_alt A A' && ((B == B') || (cut B == B'))
+    | And A _ B, And A' _ B'       => no_new_alt A A' && no_new_alt B B'
+    | Goal _program Cut, snew      => (snew == OK) || (snew == sold) || (snew == cut snew)
+    | Goal _program (Call _), snew => has_cut snew || no_new_alt_aux snew
     | _, _ => false
     end.
 
@@ -165,45 +198,112 @@ Module check (U:Unif).
   Lemma cut_is_det pr : is_det (Goal pr Cut).
   Proof. 
     move=> s s1 A [? H]; inversion H; clear H; subst; try congruence.
-    + by rewrite (expanded_cut_simpl (ex_intro _ _ H5)).
+    + have := (expanded_cut_simpl (ex_intro _ _ H5)) => -> //.
     + inversion H0; clear H0; subst; simpl in *; try congruence.
       move: H3 => [] /[subst2]; inversion H4; subst; simpl in *; congruence.
   Qed.
 
-  Definition det_rule_cut (r : R) :=
-    last Cut r.(premises) == Cut.
+  Lemma has_cut_has_cut_cut {B}: has_cut B -> has_cut (cut B).
+  Proof.
+    elim:B => //=.
+    (* + by move=> A HA _ B HB /andP [] /has_cut_and_has_cut_and_cut -> /has_cut_or_has_cut_or_cut ->.
+    + by move=> A HA B HB C HC /orP [] /has_cut_and_has_cut_and_cut -> //; rewrite orbT. *)
+  Qed.
 
-  Print state.
+  (* Lemma has_cut_and_no_new_alt_has_cut_and {A B}: has_cut_and A -> no_new_alt A B -> has_cut_and B.
+  Proof.
+    elim: A B => //.
+    + move=> [] //.
+    + move=> p [] // /=.
+      move=> ? _ /orP [/orP []|] /eqP ->. /=. *)
+
+  (* Lemma has_cut_and_cut {A}: has_cut_and (cut A).
+  Proof. 
+    elim: A => //.
+    + move=> A HA _ B HB. *)
+
+  (* Lemma has_cut_cut {A} : has_cut (cut A).
+  Proof. 
+    case:A => //=.
+    + move=> /= A _ B.
+      admit.
+    + move=> /= A B C. *)
+
+  (* Lemma has_cut_and_valid {A}: has_cut_and A -> valid_state A.
+  Proof.
+    elim: A=>// A HA B HB C HC /= /orP [/[dup]/HA|/[dup]/HC] -> H. *)
 
   Lemma no_new_alt_trans {A B C}: no_new_alt A B -> no_new_alt B C -> no_new_alt A C.
   Proof.
     elim: A B C => //; try by move=> [].
     + move=> [] [] //=.
     + move=> [] [] //=.
-    + move=> /= _ _ B C.
-      elim: B C => //; try by move=> [] //.
-      + move=>  A HA s B HB  [] //= C _ D /andP [] AC /eqP HB' /andP [] CD HE.
-        by rewrite <- HB' in HE; move: HE => /orP [] /eqP <-; rewrite HB' cut_cut_same eq_refl (HA _ AC CD).
-      + by move=> A IHA B0 _ B IHB [] // C D E /= /andP [] HA HB /andP [] HA' HB'; rewrite (IHA _ HA HA') (IHB _ HB HB').
+    + move=> [] [] //=.
+    + move=> p [| _] /=.
+      + move=> B +.
+        have := orbN (B == KO) => /orP [] /eqP.
+        + move=> -> [] //.
+        + move=> H1 + H.
+          have {}H: ((B == OK) || (B == Goal p Cut) || (B == cut B)).
+            case: B H1 H => //.
+          move: H => /orP[/orP[]|] /eqP -> //; move=> [] //.
+      + move=> B + H.
+        have {H}: (B == KO) || (has_cut B || no_new_alt_aux B).
+          case: B H => //; rewrite orbT.
+        move=> /orP [/eqP|/orP []].
+        + move=> -> [] // H. 
+        + move=> H [] //.
+          + move=> ? []//.
+          + move=> ???; destruct B => //=.
+            + by destruct a => //. 
+            + move: H => /= /andP [] H1 H2 /andP [] H3 /orP [] /eqP <-; rewrite ?cut_cut_same ?H2.
+              + 
+              + 
+          + 
+        +
     + move=> A HA s B HB [] => //= C _ D [] // E _ F.
       move=> /andP [] AC HB' /andP [] CD HE .
       rewrite (HA _ _ AC CD).
       by move: HB' HE => /orP [] /eqP ? /orP [] /eqP ?; subst; try rewrite cut_cut_same; rewrite eq_refl//orbT.
     + move=> A HA B0 _ B HB [] //= ? _ ?[] //= ? _ ? /andP [] AC HB' /andP [] CD HE .
       by rewrite (HA _ _ AC CD) (HB _ _ HB' HE).
-  Qed.
-
-  Definition get_state r := match r with 
-    | Failure A | Solved _ A | CutBrothers _ A | Expanded _ A => A 
-  end.
+  Abort.
 
   Lemma no_new_alt_id {B} : no_new_alt B B.
   Proof. elim: B => //.
+    + by move=> ? [] //=; rewrite eq_refl.
     + by move=> ? H ?? H1 /=; rewrite H eq_refl.
     + by move=> ? H ? H1 ? H2 /=; rewrite H H2.
   Qed. 
 
-  Lemma expandedb_no_new_alt {A s1 r}: 
+  Lemma det_rule_cut_has_cut_and {p r1}:
+     det_rule_cut r1 -> has_cut_and (big_and p (premises r1)).
+  Proof.
+    case: r1 => hd [] /=; rewrite /det_rule_cut//=.
+    move=> + l; elim: l.
+    + move=> [] //.
+    + move=> a l IH /= a1 /IH /orP [].
+      + by case: a => [] //; rewrite orbT.
+      + by move=> ->; rewrite 2!orbT.
+  Qed.
+
+  Lemma det_rule_has_cut_or {r rs p t s}:
+    det_rule_cut r -> all det_rule_cut rs -> 
+      has_cut_or (big_or_aux p r (select t (modes p t) rs s)).
+  Proof.
+    elim: rs r s t.
+    + move=> [] // hd [] // a l; simpl big_or_aux; unfold det_rule_cut => /= _ _ + _.
+      elim: l a {hd} => [[ ]|] //=.
+      by move=> a l IH a1 /IH /orP [] ->; rewrite 2?orbT.
+    + move=> r rs IH r1 r1s t HR1 /= /andP [] HR HRs.
+      case H: H => /=; [|apply:IH => //].
+      have : has_cut_and (big_and p (premises r1)).
+        by apply: det_rule_cut_has_cut_and.
+      move=> ->.
+      by rewrite IH.
+  Qed.
+
+  Lemma expand_no_new_alt {A s1 r}: 
     (forall pr : program, all det_rule_cut (rules pr)) ->
     valid_state A -> expand s1 A = r -> no_new_alt A (get_state r).
   Proof.
@@ -215,7 +315,16 @@ Module check (U:Unif).
     + by move=> s [] // ??? [] ??/[subst] /=.
     + move=> p [] //.
       + by move=> /= * /[subst].
-      + move=> * /[subst]. admit.
+      + move=> t s r _ ? /[subst]; simpl expand; unfold big_or; simpl get_state; unfold F.
+        remember (rules p) as rp eqn:hrp.
+        have := AllCut p; rewrite <-hrp; clear hrp AllCut.
+        elim: rp s t => // [r rs] IH s t /= /andP [] Hr /[dup] Hrs /IH {}IH.
+        case Hh: H => // [a |].
+        + move=> /=; clear IH Hh a.
+          suffices: has_cut_or (big_or_aux p r (select t (modes p t) rs s)).
+          by move=> ->.
+          by apply: det_rule_has_cut_or.
+        + by have:= IH s t => /= /orP [] -> //; rewrite orbT.
     + move=> A HA s B HB s1 +; simpl valid_state => + /andP [] VA VB => -[].
       + move=> ?? /simpl_expand_or_expanded [].
         + by move=> [A'[HA']] ? /[subst] /=; rewrite eq_refl (HA _ _ VA HA').
@@ -227,16 +336,28 @@ Module check (U:Unif).
         by rewrite eq_refl (HA _ _ VA HA').
     + move=> A HA B0 _ B HB s1 +; simpl valid_state => + /andP [] /andP [] VB VA H => -[].
       + move=> ?? /simpl_expand_and_expanded [].
+        + by move=> [A'[HA']] ? /[subst] /= ; rewrite (HA _ _ VA HA') no_new_alt_id.
+        + move=> [?[?[?[HA'[HB']]]]] ? /[subst] /=.
+          move: H; case success.
+          + by move=> {}VB; rewrite (HA _ _ VA HA') (HB _ _ VB HB').
+          + by move=> /eqP HB0; rewrite HB0 in VB; rewrite (HA _ _ VA HA') (HB _ _ (base_and_base_and_ko_valid VB) HB').
+      + move=> ?? /simpl_expand_and_cut => -[].
         + by move=> [A'[HA']] ? /[subst] /=; rewrite (HA _ _ VA HA') no_new_alt_id.
         + move=> [?[?[?[HA'[HB']]]]] ? /[subst] /=.
           move: H; case success.
           + by move=> {}VB; rewrite (HA _ _ VA HA') (HB _ _ VB HB').
           + by move=> /eqP HB0; rewrite HB0 in VB; rewrite (HA _ _ VA HA') (HB _ _ (base_and_base_and_ko_valid VB) HB').
-      + move=> ?? /simpl_expand_and_cut.
-        admit.
-      + move=> ? /simpl_expand_and_fail. admit.
-      + move=> ?? /simpl_expand_and_solved. admit.
-  Abort.
+      + move=> ? /simpl_expand_and_fail -[].
+        + by move=> [A'[HA']] ?/[subst] /=; rewrite (HA _ _ VA HA') no_new_alt_id.
+        + move=> [?[?[?[HA'[HB']]]]] ? /[subst] /=.
+          move: H; case success.
+          + by move=> {}VB; rewrite (HA _ _ VA HA') (HB _ _ VB HB').
+          + by move=> /eqP HB0; rewrite HB0 in VB; rewrite (HA _ _ VA HA') (HB _ _ (base_and_base_and_ko_valid VB) HB').
+      + move=> ?? /simpl_expand_and_solved [?[A'[B'[HA'[HB']]]]] ?/[subst] /=.
+        move: H; case success.
+        + by move=> {}VB; rewrite (HA _ _ VA HA') (HB _ _ VB HB').
+        + by move=> /eqP HB0; rewrite HB0 in VB; rewrite (HA _ _ VA HA') (HB _ _ (base_and_base_and_ko_valid VB) HB').
+  Qed.
 
 
   Lemma expandedb_no_new_alt {A B s1 b1}: 
@@ -246,7 +367,13 @@ Module check (U:Unif).
     move=> AllCut.
     remember (Failed _) as RF eqn:HRF.
     move=> + H; elim: H B HRF => //; clear -AllCut.
-    + move=> s2 A B HA ? [] <-.
+    + move=> s2 A B HA ? [] <- VA.
+      by have := expand_no_new_alt AllCut VA HA.
+    + move=> s1 s2 r A B b /[dup] H /valid_state_cb HA HE IH C ? /[subst] /[dup] VA /HA VB.
+      have NA := expand_no_new_alt AllCut VA H.
+      have NB := IH _ erefl VB.
+      apply: no_new_alt_trans.
+
   Abort.
 
   Lemma tail_cut_is_det A :
